permutationQuotientContribution low ~ mid

src/specs/PermutationQuotientContribution.ec
@@ -5,41 +5,63 @@ require import PurePrimops.
 require import UInt256.
 require import Verifier.
 require import YulPrimops.
+require import Utils.
+require        VerifierConsts.
+require        VerifierVars.
+require        VerifierMem.
+
+import VerifierConsts VerifierVars.
 
 module PermutationQuotientContribution = {
   proc low(): uint256 = {
-    var usr_res, _3, _5, usr_gamma, usr_beta, usr_factorMultiplier, _9, _11, _13, _15, _17, _19, tmp280, _22, usr_l0AtZ, tmp282;
-    _3 <@ Primops.mload(W256.of_int 2848);
-    _5 <@ Primops.mload(W256.of_int 3680);
-    usr_res <- (PurePrimops.mulmod _5 _3 (W256.of_int Constants.R));
-    usr_gamma <@ Primops.mload(W256.of_int 3584);
-    usr_beta <@ Primops.mload(W256.of_int 3552);
-    _9 <@ Primops.mload(W256.of_int 2752);
-    usr_factorMultiplier <- (PurePrimops.mulmod _9 usr_beta (W256.of_int Constants.R));
+    var usr_res, tmp270, tmp271, usr_gamma, usr_beta, usr_factorMultiplier, tmp274, tmp275, tmp276, tmp277, tmp278, tmp279, tmp280, _22, usr_l0AtZ, tmp282, _26;
+    tmp270 <@ Primops.mload(STATE_POWER_OF_ALPHA_4_SLOT);
+    tmp271 <@ Primops.mload(PROOF_COPY_PERMUTATION_GRAND_PRODUCT_OPENING_AT_Z_OMEGA_SLOT);
+    usr_res <- (PurePrimops.mulmod tmp271 tmp270 (W256.of_int Constants.R));
+    usr_gamma <@ Primops.mload(STATE_GAMMA_SLOT);
+    usr_beta <@ Primops.mload(STATE_BETA_SLOT);
+    tmp274 <@ Primops.mload(PROOF_COPY_PERMUTATION_POLYS_0_OPENING_AT_Z_SLOT);
+    usr_factorMultiplier <- (PurePrimops.mulmod tmp274 usr_beta (W256.of_int Constants.R));
     usr_factorMultiplier <- (PurePrimops.addmod usr_factorMultiplier usr_gamma (W256.of_int Constants.R));
-    _11 <@ Primops.mload(W256.of_int 2560);
-    usr_factorMultiplier <- (PurePrimops.addmod usr_factorMultiplier _11 (W256.of_int Constants.R));
+    tmp275 <@ Primops.mload(PROOF_STATE_POLYS_0_OPENING_AT_Z_SLOT);
+    usr_factorMultiplier <- (PurePrimops.addmod usr_factorMultiplier tmp275 (W256.of_int Constants.R));
     usr_res <- (PurePrimops.mulmod usr_res usr_factorMultiplier (W256.of_int Constants.R));
-    _13 <@ Primops.mload(W256.of_int 2784);
-    usr_factorMultiplier <- (PurePrimops.mulmod _13 usr_beta (W256.of_int Constants.R));
+    tmp276 <@ Primops.mload(PROOF_COPY_PERMUTATION_POLYS_1_OPENING_AT_Z_SLOT);
+    usr_factorMultiplier <- (PurePrimops.mulmod tmp276 usr_beta (W256.of_int Constants.R));
     usr_factorMultiplier <- (PurePrimops.addmod usr_factorMultiplier usr_gamma (W256.of_int Constants.R));
-    _15 <@ Primops.mload(W256.of_int 2592);
-    usr_factorMultiplier <- (PurePrimops.addmod usr_factorMultiplier _15 (W256.of_int Constants.R));
+    tmp277 <@ Primops.mload(PROOF_STATE_POLYS_1_OPENING_AT_Z_SLOT);
+    usr_factorMultiplier <- (PurePrimops.addmod usr_factorMultiplier tmp277 (W256.of_int Constants.R));
     usr_res <- (PurePrimops.mulmod usr_res usr_factorMultiplier (W256.of_int Constants.R));
-    _17 <@ Primops.mload(W256.of_int 2816);
-    usr_factorMultiplier <- (PurePrimops.mulmod _17 usr_beta (W256.of_int Constants.R));
+    tmp278 <@ Primops.mload(PROOF_COPY_PERMUTATION_POLYS_2_OPENING_AT_Z_SLOT);
+    usr_factorMultiplier <- (PurePrimops.mulmod tmp278 usr_beta (W256.of_int Constants.R));
     usr_factorMultiplier <- (PurePrimops.addmod usr_factorMultiplier usr_gamma (W256.of_int Constants.R));
-    _19 <@ Primops.mload(W256.of_int 2624);
-    usr_factorMultiplier <- (PurePrimops.addmod usr_factorMultiplier _19 (W256.of_int Constants.R));
+    tmp279 <@ Primops.mload(PROOF_STATE_POLYS_2_OPENING_AT_Z_SLOT);
+    usr_factorMultiplier <- (PurePrimops.addmod usr_factorMultiplier tmp279 (W256.of_int Constants.R));
     usr_res <- (PurePrimops.mulmod usr_res usr_factorMultiplier (W256.of_int Constants.R));
-    tmp280 <@ Primops.mload(W256.of_int 2656);
+    tmp280 <@ Primops.mload(PROOF_STATE_POLYS_3_OPENING_AT_Z_SLOT);
     _22 <- (PurePrimops.addmod tmp280 usr_gamma (W256.of_int Constants.R));
-    usr_res <- ((W256.of_int Constants.R) - (PurePrimops.mulmod usr_res _22 (W256.of_int Constants.R)));
-    usr_l0AtZ <@ Primops.mload((W256.of_int 4128));
-    tmp282 <@ Primops.mload((W256.of_int 3712));
+    usr_res <- (PurePrimops.mulmod usr_res _22 (W256.of_int Constants.R));
+    usr_res <- ((W256.of_int Constants.R) - usr_res);
+    usr_l0AtZ <@ Primops.mload(STATE_L_0_AT_Z_SLOT);
+    tmp282 <@ Primops.mload(STATE_POWER_OF_ALPHA_5_SLOT);
     usr_l0AtZ <- (PurePrimops.mulmod usr_l0AtZ tmp282 (W256.of_int Constants.R));
-    usr_res <- (PurePrimops.addmod usr_res ((W256.of_int Constants.R) - usr_l0AtZ) (W256.of_int Constants.R));
+    _26 <- ((W256.of_int Constants.R) - usr_l0AtZ);
+    usr_res <- (PurePrimops.addmod usr_res _26 (W256.of_int Constants.R));
     return usr_res;
+  }
+
+  proc mid() : int = {
+    var s0BGa, s1BGb, s2BGc, s3G, inv1, inv2;
+    
+    s0BGa <- (Sigma0_z * Beta + Gamma + A_z) %% Constants.R;
+    s1BGb <- (Sigma1_z * Beta + Gamma + B_z) %% Constants.R;
+    s2BGc <- (Sigma2_z * Beta + Gamma + C_z) %% Constants.R;
+    s3G   <- (Sigma3_z + Gamma) %% Constants.R;
+
+    inv1 <- Constants.R - (Alpha4 * Zperm_zOmega * s0BGa * s1BGb * s2BGc * s3G) %% Constants.R;
+    inv2 <- Constants.R - (Alpha5 * L0_z) %% Constants.R;
+    
+    return (inv1 + inv2) %% Constants.R;
   }
 }.
 
@@ -49,12 +71,328 @@ lemma permutationQuotientContribution_extracted_equiv_low:
       ={arg, glob PermutationQuotientContribution} ==>
       ={res, glob PermutationQuotientContribution}
     ].
-    proof.
-    proc.
-      wp.
-      inline Primops.mload.
-      wp.
-      skip.
-      rewrite /Constants.R.
-      by progress.
-    qed.
+proof. proc.
+  inline *; wp; skip; progress; by smt ().
+qed. 
+
+section.
+
+local module TMP = {
+  proc low1(): uint256 = {
+    var usr_res, _alpha4, _zperm_zOmega, usr_gamma, usr_beta, usr_factorMultiplier, _sigma0_z, _a_z, _sigma1_z, _b_z, _sigma2_z, _c_z, _sigma3_z, _22, usr_l0AtZ, _alpha5, _26;
+    _alpha4 <@ Primops.mload(STATE_POWER_OF_ALPHA_4_SLOT);
+    _zperm_zOmega <@ Primops.mload(PROOF_COPY_PERMUTATION_GRAND_PRODUCT_OPENING_AT_Z_OMEGA_SLOT);
+    usr_gamma <@ Primops.mload(STATE_GAMMA_SLOT);
+    usr_beta <@ Primops.mload(STATE_BETA_SLOT);
+    _sigma0_z <@ Primops.mload(PROOF_COPY_PERMUTATION_POLYS_0_OPENING_AT_Z_SLOT);
+    _a_z <@ Primops.mload(PROOF_STATE_POLYS_0_OPENING_AT_Z_SLOT);
+    _sigma1_z <@ Primops.mload(PROOF_COPY_PERMUTATION_POLYS_1_OPENING_AT_Z_SLOT);
+    _b_z <@ Primops.mload(PROOF_STATE_POLYS_1_OPENING_AT_Z_SLOT);
+    _sigma2_z <@ Primops.mload(PROOF_COPY_PERMUTATION_POLYS_2_OPENING_AT_Z_SLOT);
+    _c_z <@ Primops.mload(PROOF_STATE_POLYS_2_OPENING_AT_Z_SLOT);
+    _sigma3_z <@ Primops.mload(PROOF_STATE_POLYS_3_OPENING_AT_Z_SLOT);
+    usr_l0AtZ <@ Primops.mload(STATE_L_0_AT_Z_SLOT);
+    _alpha5 <@ Primops.mload(STATE_POWER_OF_ALPHA_5_SLOT);
+    
+    usr_res <- (PurePrimops.mulmod _zperm_zOmega _alpha4 (W256.of_int Constants.R));
+    usr_factorMultiplier <- (PurePrimops.mulmod _sigma0_z usr_beta (W256.of_int Constants.R));
+    usr_factorMultiplier <- (PurePrimops.addmod usr_factorMultiplier usr_gamma (W256.of_int Constants.R));
+    usr_factorMultiplier <- (PurePrimops.addmod usr_factorMultiplier _a_z (W256.of_int Constants.R));
+    usr_res <- (PurePrimops.mulmod usr_res usr_factorMultiplier (W256.of_int Constants.R));
+    usr_factorMultiplier <- (PurePrimops.mulmod _sigma1_z usr_beta (W256.of_int Constants.R));
+    usr_factorMultiplier <- (PurePrimops.addmod usr_factorMultiplier usr_gamma (W256.of_int Constants.R));
+    usr_factorMultiplier <- (PurePrimops.addmod usr_factorMultiplier _b_z (W256.of_int Constants.R));
+    usr_res <- (PurePrimops.mulmod usr_res usr_factorMultiplier (W256.of_int Constants.R));
+    usr_factorMultiplier <- (PurePrimops.mulmod _sigma2_z usr_beta (W256.of_int Constants.R));
+    usr_factorMultiplier <- (PurePrimops.addmod usr_factorMultiplier usr_gamma (W256.of_int Constants.R));
+    usr_factorMultiplier <- (PurePrimops.addmod usr_factorMultiplier _c_z (W256.of_int Constants.R));
+    usr_res <- (PurePrimops.mulmod usr_res usr_factorMultiplier (W256.of_int Constants.R));
+    _22 <- (PurePrimops.addmod _sigma3_z usr_gamma (W256.of_int Constants.R));
+    usr_res <- (PurePrimops.mulmod usr_res _22 (W256.of_int Constants.R));
+    usr_res <- ((W256.of_int Constants.R) - usr_res);
+    usr_l0AtZ <- (PurePrimops.mulmod usr_l0AtZ _alpha5 (W256.of_int Constants.R));
+    _26 <- ((W256.of_int Constants.R) - usr_l0AtZ);
+    usr_res <- (PurePrimops.addmod usr_res _26 (W256.of_int Constants.R));
+    return usr_res;
+  }
+
+  proc low2(): uint256 = {
+    var usr_res, _alpha4, _zperm_zOmega, usr_gamma, usr_beta, usr_factorMultiplier, _sigma0_z, _a_z, _sigma1_z, _b_z, _sigma2_z, _c_z, _sigma3_z, usr_l0AtZ, _alpha5, _26;
+    var s0BGa, s1BGb, s2BGc, s3G;
+    
+    _alpha4 <@ Primops.mload(STATE_POWER_OF_ALPHA_4_SLOT);
+    _zperm_zOmega <@ Primops.mload(PROOF_COPY_PERMUTATION_GRAND_PRODUCT_OPENING_AT_Z_OMEGA_SLOT);
+    usr_gamma <@ Primops.mload(STATE_GAMMA_SLOT);
+    usr_beta <@ Primops.mload(STATE_BETA_SLOT);
+    _sigma0_z <@ Primops.mload(PROOF_COPY_PERMUTATION_POLYS_0_OPENING_AT_Z_SLOT);
+    _a_z <@ Primops.mload(PROOF_STATE_POLYS_0_OPENING_AT_Z_SLOT);
+    _sigma1_z <@ Primops.mload(PROOF_COPY_PERMUTATION_POLYS_1_OPENING_AT_Z_SLOT);
+    _b_z <@ Primops.mload(PROOF_STATE_POLYS_1_OPENING_AT_Z_SLOT);
+    _sigma2_z <@ Primops.mload(PROOF_COPY_PERMUTATION_POLYS_2_OPENING_AT_Z_SLOT);
+    _c_z <@ Primops.mload(PROOF_STATE_POLYS_2_OPENING_AT_Z_SLOT);
+    _sigma3_z <@ Primops.mload(PROOF_STATE_POLYS_3_OPENING_AT_Z_SLOT);
+    usr_l0AtZ <@ Primops.mload(STATE_L_0_AT_Z_SLOT);
+    _alpha5 <@ Primops.mload(STATE_POWER_OF_ALPHA_5_SLOT);
+    
+    usr_res <- (PurePrimops.mulmod _zperm_zOmega _alpha4 (W256.of_int Constants.R));
+    
+    s0BGa <- (PurePrimops.mulmod _sigma0_z usr_beta (W256.of_int Constants.R));
+    s0BGa <- (PurePrimops.addmod s0BGa usr_gamma (W256.of_int Constants.R));
+    s0BGa <- (PurePrimops.addmod s0BGa _a_z (W256.of_int Constants.R));
+
+    usr_factorMultiplier <- s0BGa;
+    usr_res <- (PurePrimops.mulmod usr_res usr_factorMultiplier (W256.of_int Constants.R));
+    
+    s1BGb <- (PurePrimops.mulmod _sigma1_z usr_beta (W256.of_int Constants.R));
+    s1BGb <- (PurePrimops.addmod s1BGb usr_gamma (W256.of_int Constants.R));
+    s1BGb <- (PurePrimops.addmod s1BGb _b_z (W256.of_int Constants.R));
+
+    usr_factorMultiplier <- s1BGb;
+    usr_res <- (PurePrimops.mulmod usr_res usr_factorMultiplier (W256.of_int Constants.R));
+
+    s2BGc <- (PurePrimops.mulmod _sigma2_z usr_beta (W256.of_int Constants.R));
+    s2BGc <- (PurePrimops.addmod s2BGc usr_gamma (W256.of_int Constants.R));
+    s2BGc <- (PurePrimops.addmod s2BGc _c_z (W256.of_int Constants.R));
+
+    usr_factorMultiplier <- s2BGc;
+    usr_res <- (PurePrimops.mulmod usr_res usr_factorMultiplier (W256.of_int Constants.R));
+
+    s3G   <- (PurePrimops.addmod _sigma3_z usr_gamma (W256.of_int Constants.R));
+    usr_res <- (PurePrimops.mulmod usr_res s3G (W256.of_int Constants.R));
+    
+    usr_res <- ((W256.of_int Constants.R) - usr_res);
+    usr_l0AtZ <- (PurePrimops.mulmod usr_l0AtZ _alpha5 (W256.of_int Constants.R));
+    _26 <- ((W256.of_int Constants.R) - usr_l0AtZ);
+    usr_res <- (PurePrimops.addmod usr_res _26 (W256.of_int Constants.R));
+    return usr_res;
+  }
+
+  proc low3(): uint256 = {
+    var usr_res1, usr_res2, _alpha4, _zperm_zOmega, usr_gamma, usr_beta, _sigma0_z, _a_z, _sigma1_z, _b_z, _sigma2_z, _c_z, _sigma3_z, usr_l0AtZ, _alpha5;
+    var s0BGa, s1BGb, s2BGc, s3G;
+    var inv1, inv2;
+    
+    _alpha4 <@ Primops.mload(STATE_POWER_OF_ALPHA_4_SLOT);
+    _zperm_zOmega <@ Primops.mload(PROOF_COPY_PERMUTATION_GRAND_PRODUCT_OPENING_AT_Z_OMEGA_SLOT);
+    usr_gamma <@ Primops.mload(STATE_GAMMA_SLOT);
+    usr_beta <@ Primops.mload(STATE_BETA_SLOT);
+    _sigma0_z <@ Primops.mload(PROOF_COPY_PERMUTATION_POLYS_0_OPENING_AT_Z_SLOT);
+    _a_z <@ Primops.mload(PROOF_STATE_POLYS_0_OPENING_AT_Z_SLOT);
+    _sigma1_z <@ Primops.mload(PROOF_COPY_PERMUTATION_POLYS_1_OPENING_AT_Z_SLOT);
+    _b_z <@ Primops.mload(PROOF_STATE_POLYS_1_OPENING_AT_Z_SLOT);
+    _sigma2_z <@ Primops.mload(PROOF_COPY_PERMUTATION_POLYS_2_OPENING_AT_Z_SLOT);
+    _c_z <@ Primops.mload(PROOF_STATE_POLYS_2_OPENING_AT_Z_SLOT);
+    _sigma3_z <@ Primops.mload(PROOF_STATE_POLYS_3_OPENING_AT_Z_SLOT);
+    usr_l0AtZ <@ Primops.mload(STATE_L_0_AT_Z_SLOT);
+    _alpha5 <@ Primops.mload(STATE_POWER_OF_ALPHA_5_SLOT);
+    
+    usr_res1 <- (PurePrimops.mulmod _zperm_zOmega _alpha4 (W256.of_int Constants.R));
+    
+    s0BGa <- (PurePrimops.mulmod _sigma0_z usr_beta (W256.of_int Constants.R));
+    s0BGa <- (PurePrimops.addmod s0BGa usr_gamma (W256.of_int Constants.R));
+    s0BGa <- (PurePrimops.addmod s0BGa _a_z (W256.of_int Constants.R));
+
+    usr_res1 <- (PurePrimops.mulmod usr_res1 s0BGa (W256.of_int Constants.R));
+    
+    s1BGb <- (PurePrimops.mulmod _sigma1_z usr_beta (W256.of_int Constants.R));
+    s1BGb <- (PurePrimops.addmod s1BGb usr_gamma (W256.of_int Constants.R));
+    s1BGb <- (PurePrimops.addmod s1BGb _b_z (W256.of_int Constants.R));
+
+    usr_res1 <- (PurePrimops.mulmod usr_res1 s1BGb (W256.of_int Constants.R));
+
+    s2BGc <- (PurePrimops.mulmod _sigma2_z usr_beta (W256.of_int Constants.R));
+    s2BGc <- (PurePrimops.addmod s2BGc usr_gamma (W256.of_int Constants.R));
+    s2BGc <- (PurePrimops.addmod s2BGc _c_z (W256.of_int Constants.R));
+
+    usr_res1 <- (PurePrimops.mulmod usr_res1 s2BGc (W256.of_int Constants.R));
+
+    s3G   <- (PurePrimops.addmod _sigma3_z usr_gamma (W256.of_int Constants.R));
+    usr_res1 <- (PurePrimops.mulmod usr_res1 s3G (W256.of_int Constants.R));
+    inv1 <- ((W256.of_int Constants.R) - usr_res1);
+    
+    usr_res2 <- (PurePrimops.mulmod usr_l0AtZ _alpha5 (W256.of_int Constants.R));
+    inv2 <- ((W256.of_int Constants.R) - usr_res2);
+
+    return (PurePrimops.addmod inv1 inv2 (W256.of_int Constants.R));
+  }
+
+  proc low4(): uint256 = {
+    var usr_res1, usr_res2, _alpha4, _zperm_zOmega, usr_gamma, usr_beta, _sigma0_z, _a_z, _sigma1_z, _b_z, _sigma2_z, _c_z, _sigma3_z, usr_l0AtZ, _alpha5;
+    var s0BGa, s1BGb, s2BGc, s3G;
+    var inv1, inv2;
+    
+    _alpha4 <@ Primops.mload(STATE_POWER_OF_ALPHA_4_SLOT);
+    _zperm_zOmega <@ Primops.mload(PROOF_COPY_PERMUTATION_GRAND_PRODUCT_OPENING_AT_Z_OMEGA_SLOT);
+    usr_gamma <@ Primops.mload(STATE_GAMMA_SLOT);
+    usr_beta <@ Primops.mload(STATE_BETA_SLOT);
+    _sigma0_z <@ Primops.mload(PROOF_COPY_PERMUTATION_POLYS_0_OPENING_AT_Z_SLOT);
+    _a_z <@ Primops.mload(PROOF_STATE_POLYS_0_OPENING_AT_Z_SLOT);
+    _sigma1_z <@ Primops.mload(PROOF_COPY_PERMUTATION_POLYS_1_OPENING_AT_Z_SLOT);
+    _b_z <@ Primops.mload(PROOF_STATE_POLYS_1_OPENING_AT_Z_SLOT);
+    _sigma2_z <@ Primops.mload(PROOF_COPY_PERMUTATION_POLYS_2_OPENING_AT_Z_SLOT);
+    _c_z <@ Primops.mload(PROOF_STATE_POLYS_2_OPENING_AT_Z_SLOT);
+    _sigma3_z <@ Primops.mload(PROOF_STATE_POLYS_3_OPENING_AT_Z_SLOT);
+    usr_l0AtZ <@ Primops.mload(STATE_L_0_AT_Z_SLOT);
+    _alpha5 <@ Primops.mload(STATE_POWER_OF_ALPHA_5_SLOT);
+    
+    s0BGa <- (PurePrimops.mulmod _sigma0_z usr_beta (W256.of_int Constants.R));
+    s0BGa <- (PurePrimops.addmod s0BGa usr_gamma (W256.of_int Constants.R));
+    s0BGa <- (PurePrimops.addmod s0BGa _a_z (W256.of_int Constants.R));
+    
+    s1BGb <- (PurePrimops.mulmod _sigma1_z usr_beta (W256.of_int Constants.R));
+    s1BGb <- (PurePrimops.addmod s1BGb usr_gamma (W256.of_int Constants.R));
+    s1BGb <- (PurePrimops.addmod s1BGb _b_z (W256.of_int Constants.R));
+
+    s2BGc <- (PurePrimops.mulmod _sigma2_z usr_beta (W256.of_int Constants.R));
+    s2BGc <- (PurePrimops.addmod s2BGc usr_gamma (W256.of_int Constants.R));
+    s2BGc <- (PurePrimops.addmod s2BGc _c_z (W256.of_int Constants.R));
+
+    s3G   <- (PurePrimops.addmod _sigma3_z usr_gamma (W256.of_int Constants.R));
+
+    usr_res1 <- (PurePrimops.mulmod _zperm_zOmega _alpha4 (W256.of_int Constants.R));
+    usr_res1 <- (PurePrimops.mulmod usr_res1 s0BGa (W256.of_int Constants.R));
+    usr_res1 <- (PurePrimops.mulmod usr_res1 s1BGb (W256.of_int Constants.R));
+    usr_res1 <- (PurePrimops.mulmod usr_res1 s2BGc (W256.of_int Constants.R));
+    usr_res1 <- (PurePrimops.mulmod usr_res1 s3G (W256.of_int Constants.R));
+    inv1 <- ((W256.of_int Constants.R) - usr_res1);
+    
+    usr_res2 <- (PurePrimops.mulmod usr_l0AtZ _alpha5 (W256.of_int Constants.R));
+    inv2 <- ((W256.of_int Constants.R) - usr_res2);
+
+    return (PurePrimops.addmod inv1 inv2 (W256.of_int Constants.R));
+  }
+}.
+
+
+local lemma low_equiv_low1 :
+equiv [PermutationQuotientContribution.low ~ TMP.low1 :
+      ={arg, Primops.memory} ==> ={res, Primops.memory}].
+proof. proc.
+  inline *; wp; skip; progress; smt ().
+qed.
+
+local lemma low1_equiv_low2 :
+     equiv [TMP.low1 ~ TMP.low2 : ={arg, glob TMP} ==> ={res, glob TMP}].
+proof. proc.
+  inline *; wp; skip; progress; smt ().
+qed.
+
+local lemma low2_equiv_low3 :
+     equiv [TMP.low2 ~ TMP.low3 : ={arg, glob TMP} ==> ={res, glob TMP}].
+proof. proc.
+  inline *; wp; skip; progress; smt ().
+qed.
+
+local lemma low3_equiv_low4 :
+     equiv [TMP.low3 ~ TMP.low4 : ={arg, glob TMP} ==> ={res, glob TMP}].
+proof. proc.
+  inline *; wp; skip; progress; smt ().
+qed.
+
+local lemma low_equiv_low4 :
+equiv [PermutationQuotientContribution.low ~ TMP.low4 :
+      ={arg, Primops.memory} ==> ={res, Primops.memory}].
+proof.
+transitivity TMP.low1 (={arg, glob PermutationQuotientContribution} ==> ={res, glob PermutationQuotientContribution}) (={arg, Primops.memory} ==> ={res, Primops.memory}); progress.
+exists Primops.memory{2}. progress. apply low_equiv_low1.
+transitivity TMP.low2 (={arg, glob TMP} ==> ={res, glob TMP}) (={arg, glob TMP} ==> ={res, glob TMP}); progress.
+exists Primops.memory{2}. progress. apply low1_equiv_low2.
+transitivity TMP.low3 (={arg, glob TMP} ==> ={res, glob TMP}) (={arg, glob TMP} ==> ={res, glob TMP}); progress.
+exists Primops.memory{2}. progress. apply low2_equiv_low3.
+apply low3_equiv_low4.
+qed.
+
+import MemoryMap VerifierMem.
+declare op m : mem.
+
+pred permutationQuotientContribution_pre_mem = 
+  alpha4_mem m /\ alpha5_mem m /\ beta_mem m /\ gamma_mem m /\
+  sigma0_z_mem m /\ sigma1_z_mem m /\ sigma2_z_mem m /\ sigma3_z_mem m /\
+  a_z_mem m /\ b_z_mem m /\ c_z_mem m /\  
+  zperm_zOmega_mem m /\ l0_z_mem m.
+
+lemma low_equiv_mid :
+equiv [PermutationQuotientContribution.low ~ PermutationQuotientContribution.mid :
+   ={arg, glob PermutationQuotientContribution} /\
+   Primops.memory{1} = m /\
+   !Primops.reverted{1} /\
+   !Primops.reverted{2} /\
+   permutationQuotientContribution_pre_mem
+   ==>
+   W256.to_uint res{1} = res{2}
+ ].
+proof. 
+
+transitivity
+  TMP.low4
+  (={arg, glob PermutationQuotientContribution} ==> ={res, glob PermutationQuotientContribution})
+  (={arg, glob PermutationQuotientContribution} /\
+   Primops.memory{1} = m /\
+   !Primops.reverted{1} /\
+   !Primops.reverted{2} /\
+   permutationQuotientContribution_pre_mem
+   ==>
+   W256.to_uint res{1} = res{2}); progress.
+exists m Primops.reverted{1}; auto. apply low_equiv_low4.
+rewrite /permutationQuotientContribution_pre_mem. proc.
+
+seq 13 0 : (#pre /\
+  W256.to_uint _alpha4{1} = Alpha4 /\
+  W256.to_uint _alpha5{1} = Alpha5 /\
+  W256.to_uint _zperm_zOmega{1} = Zperm_zOmega /\
+  W256.to_uint usr_gamma{1} = Gamma /\ 
+  W256.to_uint usr_beta{1} = Beta /\
+  W256.to_uint _sigma0_z{1} = Sigma0_z /\
+  W256.to_uint _sigma1_z{1} = Sigma1_z /\
+  W256.to_uint _sigma2_z{1} = Sigma2_z /\
+  W256.to_uint _sigma3_z{1} = Sigma3_z /\
+  W256.to_uint _a_z{1} = A_z /\
+  W256.to_uint _c_z{1} = C_z /\
+  W256.to_uint _b_z{1} = B_z /\
+  W256.to_uint usr_l0AtZ{1} = L0_z).
+call{1} (ConcretePrimops.mload_pspec m STATE_POWER_OF_ALPHA_5_SLOT).
+call{1} (ConcretePrimops.mload_pspec m STATE_L_0_AT_Z_SLOT).
+call{1} (ConcretePrimops.mload_pspec m PROOF_STATE_POLYS_3_OPENING_AT_Z_SLOT).
+call{1} (ConcretePrimops.mload_pspec m PROOF_STATE_POLYS_2_OPENING_AT_Z_SLOT).
+call{1} (ConcretePrimops.mload_pspec m PROOF_COPY_PERMUTATION_POLYS_2_OPENING_AT_Z_SLOT).
+call{1} (ConcretePrimops.mload_pspec m PROOF_STATE_POLYS_1_OPENING_AT_Z_SLOT).
+call{1} (ConcretePrimops.mload_pspec m PROOF_COPY_PERMUTATION_POLYS_1_OPENING_AT_Z_SLOT).
+call{1} (ConcretePrimops.mload_pspec m PROOF_STATE_POLYS_0_OPENING_AT_Z_SLOT).
+call{1} (ConcretePrimops.mload_pspec m PROOF_COPY_PERMUTATION_POLYS_0_OPENING_AT_Z_SLOT).
+call{1} (ConcretePrimops.mload_pspec m STATE_BETA_SLOT).
+call{1} (ConcretePrimops.mload_pspec m STATE_GAMMA_SLOT).
+call{1} (ConcretePrimops.mload_pspec m PROOF_COPY_PERMUTATION_GRAND_PRODUCT_OPENING_AT_Z_OMEGA_SLOT).
+call{1} (ConcretePrimops.mload_pspec m STATE_POWER_OF_ALPHA_4_SLOT).
+skip; by progress.
+
+seq 10 4 : (#pre /\ W256.to_uint s0BGa{1} = s0BGa{2} /\ W256.to_uint s1BGb{1} = s1BGb{2} /\ W256.to_uint s2BGc{1} = s2BGc{2} /\ W256.to_uint s2BGc{1} = s2BGc{2} /\ W256.to_uint s3G{1} = s3G{2}).
+wp; skip; rewrite /addmod /mulmod; progress; rewrite !W256.of_uintK; by smt().
+
+seq 5 0 : (#pre /\ W256.to_uint usr_res1{1} = (Alpha4 * Zperm_zOmega * s0BGa{2} * s1BGb{2} * s2BGc{2} * s3G{2}) %% Constants.R).
+wp; skip; rewrite /addmod /mulmod; progress; rewrite !W256.of_uintK !R_mod_W256_R !mod_R_W256_mod_R; by smt().
+
+seq 1 1 : (#pre /\ W256.to_uint inv1{1} = inv1{2}).
+wp; skip; progress; rewrite -H27.
+have ->:
+ (Constants.R - to_uint usr_res1{1}) = (Constants.R - to_uint usr_res1{1}) %% W256.modulus.
+ by smt().
+rewrite -W256.of_uintK; by smt(@W256).
+
+seq 1 0 : (#pre /\ W256.to_uint usr_res2{1} = (Alpha5 * L0_z) %% Constants.R).
+wp; skip; rewrite /addmod /mulmod; progress; rewrite !W256.of_uintK !R_mod_W256_R !mod_R_W256_mod_R; by smt().
+
+seq 1 1 : (#pre /\ W256.to_uint inv2{1} = inv2{2}).
+wp; skip; progress; rewrite -H28.
+have ->:
+ (Constants.R - to_uint usr_res2{1}) = (Constants.R - to_uint usr_res2{1}) %% W256.modulus.
+ by smt().
+rewrite -W256.of_uintK; by smt(@W256).
+
+skip; rewrite /addmod; progress; rewrite !W256.of_uintK !R_mod_W256_R !mod_R_W256_mod_R; 
+by reflexivity.
+
+qed. 
+
+end section.
+
+print low_equiv_mid.
