src/VerifierMem.ec
@@ -1,0 +1,38 @@
+require import AllCore.
+require import Int.
+require import IntDiv.
+require import UInt256.
+require import Memory.
+require import PurePrimops.
+require        VerifierConsts.
+require        VerifierVars.
+
+section.
+import VerifierConsts VerifierVars.
+
+declare op memory : MemoryMap.mem.
+
+pred alpha2_mem = W256.to_uint (PurePrimops.mload memory STATE_POWER_OF_ALPHA_2_SLOT) = Alpha2.
+pred alpha3_mem = W256.to_uint (PurePrimops.mload memory STATE_POWER_OF_ALPHA_3_SLOT) = Alpha3.
+pred alpha4_mem = W256.to_uint (PurePrimops.mload memory STATE_POWER_OF_ALPHA_4_SLOT) = Alpha4.
+pred alpha5_mem = W256.to_uint (PurePrimops.mload memory STATE_POWER_OF_ALPHA_5_SLOT) = Alpha5.
+pred alpha6_mem = W256.to_uint (PurePrimops.mload memory STATE_POWER_OF_ALPHA_6_SLOT) = Alpha6.
+pred alpha7_mem = W256.to_uint (PurePrimops.mload memory STATE_POWER_OF_ALPHA_7_SLOT) = Alpha7.
+pred alpha8_mem = W256.to_uint (PurePrimops.mload memory STATE_POWER_OF_ALPHA_8_SLOT) = Alpha8.
+
+pred beta_mem = W256.to_uint (PurePrimops.mload memory STATE_GAMMA_SLOT) = Gamma.
+pred gamma_mem = W256.to_uint (PurePrimops.mload memory STATE_BETA_SLOT) = Beta.
+
+pred sigma0_z_mem = W256.to_uint (PurePrimops.mload memory PROOF_COPY_PERMUTATION_POLYS_0_OPENING_AT_Z_SLOT) = Sigma0_z.
+pred sigma1_z_mem = W256.to_uint (PurePrimops.mload memory PROOF_COPY_PERMUTATION_POLYS_1_OPENING_AT_Z_SLOT) = Sigma1_z.
+pred sigma2_z_mem = W256.to_uint (PurePrimops.mload memory PROOF_COPY_PERMUTATION_POLYS_2_OPENING_AT_Z_SLOT) = Sigma2_z.
+pred sigma3_z_mem = W256.to_uint (PurePrimops.mload memory PROOF_STATE_POLYS_3_OPENING_AT_Z_SLOT) = Sigma3_z.
+
+pred a_z_mem = W256.to_uint (PurePrimops.mload memory PROOF_STATE_POLYS_0_OPENING_AT_Z_SLOT) = A_z.
+pred b_z_mem = W256.to_uint (PurePrimops.mload memory PROOF_STATE_POLYS_1_OPENING_AT_Z_SLOT) = B_z.
+pred c_z_mem = W256.to_uint (PurePrimops.mload memory PROOF_STATE_POLYS_2_OPENING_AT_Z_SLOT) = C_z.
+
+pred zperm_zOmega_mem = W256.to_uint (PurePrimops.mload memory PROOF_COPY_PERMUTATION_GRAND_PRODUCT_OPENING_AT_Z_OMEGA_SLOT) = Zperm_zOmega.
+pred l0_z_mem = W256.to_uint (PurePrimops.mload memory STATE_L_0_AT_Z_SLOT) = L0_z.
+
+end section.
